spot/GC.SPOT.HeapExpansion.fst
@@ -1050,6 +1050,41 @@ let spot_chunked_gc_postcondition_single_chunk_from_dense
   =
   ChunkedMajorGCCorr.chunked_gc_postcondition_single_chunk_from_dense g
 
+let spot_chunked_major_gc_bounded_single_chunk_postcondition
+  (g: heap)
+  (roots: Seq.seq obj_addr)
+  (fp: U64.t)
+  (cap: nat{cap > 0})
+  (fuel: nat)
+  : Lemma
+      (requires
+        Fields.well_formed_heap g /\
+        Seq.length (Fields.objects zero_addr g) > 0 /\
+        GC.Spec.SweepInv.heap_objects_dense g /\
+        Mark.root_props g roots /\
+        SpecSweep.fp_in_heap fp g /\
+        Mark.no_black_objects g /\
+        Mark.no_pointer_to_blue g /\
+        Fields.no_scan_invariant g /\
+        fuel >= BMark.count_non_black g /\
+        ChunkedMarkBoundedOuter.mark_bounded_single_chunk_ready
+          g cap fuel /\
+        (forall (x: obj_addr). Seq.mem x (Fields.objects zero_addr g) /\
+          (Obj.is_gray x g \/ Obj.is_black x g) ==> Seq.mem x roots) /\
+        (let graph = GC.Spec.HeapModel.create_graph g in
+         let roots' = GC.Spec.HeapGraph.coerce_to_vertex_list roots in
+         GC.Spec.Graph.graph_wf graph /\
+         GC.Spec.Graph.is_vertex_set roots' /\
+         GC.Spec.Graph.subset_vertices roots' graph.vertices))
+      (ensures
+        (let (mh_final, fp_final) =
+           ChunkedMajorGC.chunked_major_gc_bounded
+             (MH.single_chunk_major_heap g) cap fuel in
+         ChunkedMajorGCCorr.chunked_gc_postcondition mh_final))
+  =
+  ChunkedMajorGCCorr.chunked_major_gc_bounded_single_chunk_postcondition
+    g roots fp cap fuel
+
 let spot_chunked_mark_aux_empty_single_chunk_compat
   (g: heap)
   (st: Seq.seq obj_addr)
